wip: writing eo-fin proof

fairness/lawyer/eo_fin.v
@@ -1,13 +1,55 @@
 From iris.proofmode Require Import tactics coq_tactics.
-(* From iris.algebra Require Import auth gmap gset excl. *)
+From iris.algebra Require Import auth gmap gset excl excl_auth.
 (* From iris.base_logic Require Export gen_heap. *)
 (* From trillium.program_logic Require Export weakestpre adequacy ectx_lifting. *)
+From iris.base_logic.lib Require Import invariants.
 From trillium.fairness Require Import locales_helpers utils.
 From trillium.fairness.lawyer Require Import obligations_model obls_utils obligations_resources program_logic.
 From trillium.fairness.heap_lang Require Export heap_lang_defs tactics notation sswp_logic locales_helpers_hl.
 
 
 Close Scope Z.
+
+(* TODO: move *)
+Section Arithmetic.
+
+  Lemma even_succ_negb n: Nat.even (S n) = negb $ Nat.even n.
+  Proof.
+    rewrite Nat.even_succ.
+    rewrite -Nat.negb_even.
+    done. 
+  Qed.
+
+  (* Lemma odd_succ_negb n: Nat.odd (S n) = negb $ Nat.odd n. *)
+  (* Proof. by rewrite Nat.odd_succ Nat.negb_odd. Qed. *)
+
+  (* Lemma even_plus1_negb n: Nat.even (n + 1) = negb $ Nat.even n. *)
+  (* Proof. by rewrite Nat.add_1_r even_succ_negb. Qed.  *)
+
+  (* Lemma odd_plus1_negb n: Nat.odd (n + 1) = negb $ Nat.odd n. *)
+  (* Proof. by rewrite Nat.add_1_r odd_succ_negb. Qed. *)
+
+  (* Lemma even_odd_False n : Nat.even n → Nat.odd n → False. *)
+  (* Proof. *)
+  (*   intros Heven Hodd. rewrite -Nat.negb_odd in Heven. *)
+  (*   apply Is_true_true_1 in Heven. *)
+  (*   apply Is_true_true_1 in Hodd. *)
+  (*   by rewrite Hodd in Heven. *)
+  (* Qed. *)
+  
+  (* Lemma even_not_odd n : Nat.even n → ¬ Nat.odd n. *)
+  (* Proof. intros Heven Hodd. by eapply even_odd_False. Qed. *)
+  
+  (* Lemma odd_not_even n : Nat.odd n → ¬ Nat.even n. *)
+  (* Proof. intros Heven Hodd. by eapply even_odd_False. Qed. *)
+  
+  Lemma even_or_odd n: Nat.even n \/ Nat.odd n.
+  Proof. 
+    destruct (decide (Nat.even n)) as [| O]; auto.
+    apply negb_prop_intro in O. rewrite Nat.negb_even in O. tauto.
+  Qed.
+
+End Arithmetic.
 
 (* Definition EODegree n := Fin.t (S n). *)
 (* Definition EOLevel n := Fin.t (S n). *)
@@ -17,8 +59,9 @@ Definition EOLevel n := { i | i < n }.
 Section EoFin.
   Context (LIM: nat).
   Let MAX_OBL_STEPS := 10.
+  Let NUM_DEG := 5.
   
-  Instance EO_OP: ObligationsParams (EODegree LIM) (EOLevel LIM) (locale heap_lang) MAX_OBL_STEPS.
+  Instance EO_OP: ObligationsParams (EODegree NUM_DEG) (EOLevel LIM) (locale heap_lang) MAX_OBL_STEPS.
   Proof using.
     esplit; try by apply _.
     - rewrite /EODegree.
@@ -28,8 +71,8 @@ Section EoFin.
 
   Let OM := ObligationsModel EO_OP.
 
-  Let EODegreeOfe := sigO (fun i => i < LIM). 
   Let EOLevelOfe := sigO (fun i => i < LIM).
+  Let EODegreeOfe := sigO (fun i => i < NUM_DEG). 
 
   Instance foo: LeibnizEquiv EOLevelOfe.
   Admitted. 
@@ -39,7 +82,181 @@ Section EoFin.
   Context `{hGS: @heapGS Σ _ EM}.
   Let oGS : ObligationsGS EO_OP Σ := heap_fairnessGS (heapGS := hGS).
 
-  
+  Let thread_prog: val :=
+    rec: "thread_prog" "l" "n" "M" :=
+      if: ("M" ≤ "n")%V then #()
+      else                           
+        if: CAS "l" "n" ("n"+#1)
+        then "thread_prog" "l" ("n" + #2) "M"
+        else "thread_prog" "l" "n" "M"
+  .
 
+  Definition start: val :=
+    λ: "i" "M",
+      (let: "l" := Alloc "i" in
+      (Fork (thread_prog "l" "i" "M" ) ;;
+       Fork (thread_prog "l" ("i" + #1) "M")))
+  .
+
+  Class EoFinPreG Σ := {
+      eofin_threads_PreG :> inG Σ (excl_authR (prodR natO positiveO));
+      (* TODO: abstract over signal id type? *)
+      eofin_sigs :> inG Σ (excl_authR natO);
+      eofin_toks :> inG Σ (exclR unitO);
+  }.
+  
+  Class EoFinG Σ := {
+      eofin_PreG :> EoFinPreG Σ;
+      eofin_even: gname; eofin_odd: gname; 
+      eofin_p1: gname; eofin_p2: gname;
+      eofin_tok_p1: gname; eofin_tok_p2: gname;
+  }.
+
+  Section Threads.
+    Context `{EoFinG Σ}.
+    
+    Definition thread_auth γ (n: nat) (g: gname): iProp Σ :=
+      own γ (●E (n, g)).
+
+    Definition thread_frag γ (n: nat) (g: gname): iProp Σ :=
+      own γ (◯E (n, g)).
+
+    Lemma thread_agree γ n1 g1 n2 g2:
+      thread_auth γ n1 g1 -∗ thread_frag γ n2 g2 -∗ ⌜ n1 = n2 /\ g1 = g2 ⌝. 
+    Proof.
+      rewrite /thread_frag /thread_auth.
+      iIntros "HA HB". iCombine "HB HA" as "H".      
+      iDestruct (own_valid with "H") as "%Hval".
+      iPureIntro. apply excl_auth_agree_L in Hval. set_solver. 
+    Qed.
+
+    Lemma thread_update γ n1 g1 n2 g2 n' g':
+      thread_auth γ n1 g1 -∗ thread_frag γ n2 g2 ==∗
+      thread_auth γ n' g' ∗ thread_frag γ n' g'. 
+    Proof.
+      rewrite /thread_frag /thread_auth.
+      iIntros "HA HB". iCombine "HB HA" as "H".
+      rewrite -!own_op. iApply own_update; [| by iFrame].
+      apply excl_auth_update.
+    Qed.
+
+    Definition nth_lvl (n: nat) {M: nat} (BOUND: M < LIM) (LE: n <= M): EOLevel LIM :=
+      exist _ n (Nat.le_lt_trans _ _ _ LE BOUND).
+
+    Definition nth_lvl' (n: nat) {M: nat} (BOUND: M < LIM) (LE: n < M): EOLevel LIM :=
+      (* exist _ n (Nat.lt_trans _ _ _ LE BOUND). *)
+      nth_lvl n BOUND (Nat.lt_le_incl _ _ LE). 
+
+    Definition nth_deg (n: nat) (LT: n < NUM_DEG): EODegree NUM_DEG :=
+      exist _ n LT. 
+
+    Definition sgn_p_auth γ g: iProp Σ := own γ (●E g).
+    Definition sgn_p_frag γ g: iProp Σ := own γ (◯E g).
+
+    Definition thread_tok γ := own γ (Excl ()). 
+
+    Definition eofin_inv_inner l M (BOUND: M < LIM) : iProp Σ :=
+      ∃ (n: nat), 
+          l ↦ #n ∗
+          thread_auth eofin_even
+            (if Nat.even n then n else n + 1)
+            (if Nat.even n then eofin_p1 else eofin_p2) ∗
+          thread_auth eofin_odd
+            (if Nat.odd n then n else n + 1)
+            (if Nat.odd n then eofin_p1 else eofin_p2) ∗
+          (∀ (LE: n + 1 <= M), ∃ sid, sgn EO_OP sid (nth_lvl (n + 1) BOUND LE) (Some false) (H3 := oGS) ∗ (∃ c, sgn_p_auth eofin_p1 c ∗ (sgn_p_frag eofin_p1 c ∨ ⌜ c = sid ⌝ ∗ thread_tok eofin_tok_p1))) ∗
+          (∀ (LE: n + 2 <= M), ∃ sid, sgn EO_OP sid (nth_lvl (n + 2) BOUND LE) (Some false) (H3 := oGS) ∗ (∃ c, sgn_p_auth eofin_p2 c ∗ (sgn_p_frag eofin_p2 c ∨ ⌜ c = sid ⌝ ∗ thread_tok eofin_tok_p2)))
+    .
+
+    Definition eofin_inv l M BOUND: iProp Σ :=
+      inv (nroot .@ "eofin") (eofin_inv_inner l M BOUND).
+
+    Let d0 := nth_deg 0 (Nat.lt_0_succ _). 
+
+    Ltac MU_burn_cp :=
+      iApply (BMU_MU with "[-PH] [$]"); [by eauto| ]; iIntros "PH";
+      iApply BMU_intro;
+      iDestruct (cp_mul_take with "CPS") as "[CPS CP]";
+      iSplitR "CP";
+      [| do 2 iExists _; iFrame; iPureIntro; reflexivity]. 
+
+    Ltac pure_step :=
+      iApply sswp_MU_wp; [done| ];
+      iApply sswp_pure_step; [done| ]; simpl;
+      iNext;
+      MU_burn_cp
+    . 
+
+    Ltac pure_step_cases := pure_step || (iApply wp_value; []) || wp_bind (RecV _ _ _ _)%V.
+    Ltac pure_steps := repeat (pure_step_cases; []). 
+
+    Lemma add1_helper {x y: nat}: x < y -> x + 1 <= y.
+    Proof. lia. Qed.
+
+    Definition even_res n: iProp Σ :=
+      ∃ g, thread_frag eofin_even n g ∗ thread_tok g. 
+
+    Lemma thread_spec τ n l M (BOUND: M < LIM) π:
+      {{{ eofin_inv l M BOUND ∗ even_res n ∗
+          cp_mul EO_OP π d0 100 (H3 := oGS) ∗ th_phase_ge EO_OP τ π (H3 := oGS) ∗
+          ((∀ (LT: n < M), ∃ s, obls EO_OP τ {[ s ]} (H3 := oGS) ∗ sgn EO_OP s (nth_lvl (n + 1) BOUND (add1_helper LT)) None (H3 := oGS)) ∧
+           (⌜ n >= M⌝ -∗ obls EO_OP τ ∅ (H3 := oGS)))
+      }}}
+        thread_prog #l #n #M @ τ
+      {{{ x, RET #x; obls EO_OP τ ∅ (H3 := oGS) }}}.
+    Proof.
+      iIntros (Φ). iIntros "(#INV & TH & CPS & PH & OB) POST".
+      rewrite /thread_prog.
+
+      wp_bind (RecV _ _ _ _)%V.
+      pure_steps.
+      wp_bind (_ ≤ _)%E.
+      pure_step. 
+
+      destruct (Nat.le_gt_cases M n).
+      { rewrite bool_decide_true; [| lia].
+        pure_steps. iApply "POST".
+        iApply "OB". done. }
+      
+      rewrite bool_decide_false; [| lia].
+      iDestruct (bi.and_elim_l with "OB") as "OB".
+      iSpecialize ("OB" $! ltac:(done)). iDestruct "OB" as (s) "[OB SIG]".
+      pure_steps.
+      wp_bind (_ + _)%E. pure_steps.  
+      wp_bind (CmpXchg _ _ _)%E.
+
+      iApply wp_atomic. 
+      iInv "INV" as ">inv" "CLOS". iModIntro.
+      rewrite {1}/eofin_inv_inner.
+      iDestruct "inv" as (m) "(L & EVEN & ODD & P1 & P2)".
+      iDestruct "TH" as (g) "[EV TOK]". 
+      iDestruct (thread_agree with "EVEN [$]") as %[<- <-].
+      destruct (even_or_odd m) as [EVEN | ODD].
+      - pose proof (Is_true_true_1 _ EVEN) as E.
+        rewrite {1 2 3 6 7 8 9 10 11}E.
+
+        iApply sswp_MU_wp; [done| ]. 
+        iApply (wp_cmpxchg_suc with "[$]"); try done.
+        { econstructor. done. }
+        iNext. iIntros "L".
+
+        iApply (BMU_MU with "[-PH] [$]"); [by eauto| ]; iIntros "PH". 
+
+        iApply OU_BMU.
+        iDestruct (OU_set_sig with "OB [SIG]") as "OU".
+        { apply elem_of_singleton. reflexivity. }
+        { iApply "SIG". 
+        iApply (OU_wand with "[-OU]"); [| done].
+        iIntros "(SIG & OBLS)".
+
+        iMod ("CLOS" with "P2 EVEN ODD") as "_"
+
+      
+
+      
+
+
+
+  End Threads.
 
 End EoFin.
